Manual/IO.lean
@@ -1,0 +1,547 @@
+/-
+Copyright (c) 2024 Lean FRO LLC. All rights reserved.
+Released under Apache 2.0 license as described in the file LICENSE.
+Author: David Thrane Christiansen
+-/
+
+import VersoManual
+
+import Manual.Meta
+import Manual.Papers
+
+import Lean.Parser.Command
+
+import Manual.IO.Console
+import Manual.IO.Files
+import Manual.IO.Threads
+import Manual.IO.Ref
+
+open Manual
+open Verso.Genre
+open Verso.Genre.Manual
+
+set_option pp.rawOnError true
+
+set_option linter.unusedVariables false
+
+#doc (Manual) "IO" =>
+%%%
+tag := "io"
+%%%
+
+
+
+Lean is a pure functional programming language.
+While Lean code is strictly evaluated at run time, the order of evaluation that is used during type checking, especially while checking {tech}[definitional equality], is formally unspecified and makes use of a number of heuristics that improve performance but are subject to change.
+This means that simply adding operations that perform side effects (such as file I/O, exceptions, or mutable references) would lead to programs in which the order of effects is unspecified.
+During type checking, even terms with free variables are reduced; this would make side effects even more difficult to predict.
+Finally, a basic principle of Lean's logic is that functions are _functions_ that map each element of the domain to a unique element of the range.
+Including side effects such as console I/O, arbitrary mutable state, or random number generation would violate this principle.
+
+```lean (show := false)
+section Model
+/-- A type -/
+axiom α : Type
+```
+
+Programs that may have side effects have a type (typically {lean}`IO α`) that distinguishes them from pure functions.
+Logically speaking, {lean}`IO` describes the sequencing and data dependencies of side effects.
+Many of the basic side effects, such as reading from files, are opaque constants from the perspective of Lean's logic.
+Others are specified by code that is logically equivalent to the run-time version.
+At run time, the compiler produces ordinary code.
+
+# Logical Model
+
+Conceptually, Lean distinguishes evaluation or reduction of terms from _execution_ of side effects.
+Term reduction is specified by rules such as {tech}[β] and {tech}[δ], which may occur anywhere at any time.
+Side effects, which must be executed in the correct order, are abstractly described in Lean's logic.
+When programs are run, the Lean runtime system is responsible for actually carrying out the described effects.
+
+
+The type {lean}`IO α` is a description of a process that, by performing side effects, should either return a value of type {lean}`α` or throw an error.
+It can be thought of as a {tech}[state monad] in which the state is the entire world.
+Just as a value of type {lean}`StateM Nat Bool` computes a {lean}`Bool` while having the ability to mutate a natural number, a value of type {lean}`IO Bool` computes a {lean}`Bool` while potentially changing the world.
+Error handling is accomplished by layering an appropriate exception monad transformer on top of this.
+
+Because the entire world can't be represented in memory, the actual implementation uses an abstract token that stands for its state.
+The Lean runtime system is responsible for providing the initial token when the program is run, and each primitive action accepts a token that represents the world and returns another when finished.
+This ensures that effects occur in the proper order, and it clearly separates the execution of side effects from the reduction semantics of Lean terms.
+
+```lean (show := false)
+end Model
+```
+
+Non-termination via general recursion is treated separately from the effects described by {name}`IO`.
+Programs that may not terminate due to infinite loops must be defined as {ref "partial-unsafe"}[`partial`] functions.
+From the logical perspective, they are treated as arbitrary constants; {name}`IO` is not needed.
+
+A very important property of {lean}`IO` is that there is no way for values to “escape”.
+Without using one of a few clearly-marked unsafe operators, programs have no way to extract a pure {lean}`Nat` from an {lean}`IO Nat`.
+This ensures that the correct ordering of side effects is preserved, and it ensures that programs that have side effects are clearly marked as such.
+
+## The `IO`, `EIO` and `BaseIO` Monads
+
+There are two monads that are typically used for programs that interact with the real world:
+
+ * Actions in {lean}`IO` may throw exceptions of type {lean}`IO.Error` or modify the world.
+ * Actions in {lean}`BaseIO` can't throw exceptions, but they can modify the world.
+
+The distinction makes it possible to tell whether exceptions are possible by looking at an action's type signature.
+{lean}`BaseIO` actions are automatically promoted to {lean}`IO` as necessary.
+
+{docstring IO}
+
+{docstring BaseIO}
+
+Both {lean}`IO` and {lean}`BaseIO` are instances of {lean}`EIO`, in which the type of errors is a parameter.
+{lean}`IO` is defined as {lean}`EIO IO.Error`, while {lean}`BaseIO` is defined as {lean}`EIO Empty`.
+In some circumstances, such as bindings to non-Lean libraries, it can be convenient to use {lean}`EIO` with a custom error type, which ensures that errors are handled at the boundaries between these and other {lean}`IO` actions.
+
+```lean (show := false)
+-- Check claim in preceding paragraph
+example : IO = EIO IO.Error := rfl
+example : BaseIO = EIO Empty := rfl
+```
+
+{docstring EIO}
+
+{docstring IO.lazyPure}
+
+{docstring BaseIO.toIO}
+
+{docstring BaseIO.toEIO}
+
+{docstring EIO.toBaseIO}
+
+{docstring EIO.toIO}
+
+{docstring EIO.toIO'}
+
+{docstring IO.toEIO}
+
+## Errors and Error Handling
+
+Error handling in the {lean}`IO` monad uses the same facilities as any other {tech}[exception monad].
+In particular, throwing and catching exceptions uses the methods of the {name}`MonadExceptOf` {tech}[type class].
+The exceptions thrown in {lean}`IO` have the type {lean}`IO.Error`.
+The constructors of this type represent the low-level errors that occur on most operating systems, such as files not existing.
+The most-used constructor is {name IO.Error.userError}`userError`, which covers all other cases and includes a string that describes the problem.
+
+{docstring IO.Error}
+
+{docstring IO.Error.toString}
+
+{docstring IO.ofExcept}
+
+{docstring EIO.catchExceptions}
+
+{docstring IO.userError}
+
+::::example "Throwing and Catching Errors"
+:::ioExample
+This program repeatedly demands a password, using exceptions for control flow.
+The syntax used for exceptions is available in all exception monads, not just {lean}`IO`.
+When an incorrect password is provided, an exception is thrown, which is caught by the loop that repeats the password check.
+A correct password allows control to proceed past the check, terminating the loop, and any other exceptions are re-thrown.
+
+```ioLean
+def accessControl : IO Unit := do
+  IO.println "What is the password?"
+  let password ← (← IO.getStdin).getLine
+  if password.trim != "secret" then
+    throw (.userError "Incorrect password")
+  else return
+
+def repeatAccessControl : IO Unit := do
+  repeat
+    try
+      accessControl
+      break
+    catch
+      | .userError "Incorrect password" =>
+        continue
+      | other =>
+        throw other
+
+def main : IO Unit := do
+  repeatAccessControl
+  IO.println "Access granted!"
+```
+
+When run with this input:
+```stdin
+publicinfo
+secondtry
+secret
+```
+
+the program emits:
+```stdout
+What is the password?
+What is the password?
+What is the password?
+Access granted!
+```
+:::
+::::
+
+### Constructing IO Errors
+
+{docstring IO.Error.mkUnsupportedOperation}
+
+{docstring IO.Error.mkUnsatisfiedConstraints}
+
+{docstring IO.Error.mkProtocolError}
+
+{docstring IO.Error.mkResourceBusy}
+
+{docstring IO.Error.mkResourceVanished}
+
+{docstring IO.Error.mkNoSuchThing}
+
+{docstring IO.Error.mkNoSuchThingFile}
+
+{docstring IO.Error.mkEofError}
+
+{docstring IO.Error.mkPermissionDenied}
+
+{docstring IO.Error.mkNoFileOrDirectory}
+
+{docstring IO.Error.mkTimeExpired}
+
+{docstring IO.Error.fopenErrorToString}
+
+{docstring IO.Error.mkAlreadyExists}
+
+{docstring IO.Error.mkInvalidArgument}
+
+{docstring IO.Error.mkHardwareFault}
+
+{docstring IO.Error.mkResourceExhausted}
+
+{docstring IO.Error.mkInappropriateType}
+
+{docstring IO.Error.mkOtherError}
+
+{docstring IO.Error.otherErrorToString}
+
+{docstring IO.Error.mkInvalidArgumentFile}
+
+{docstring IO.Error.mkResourceExhaustedFile}
+
+{docstring IO.Error.mkAlreadyExistsFile}
+
+
+{docstring IO.Error.mkIllegalOperation}
+
+{docstring IO.Error.mkPermissionDeniedFile}
+
+{docstring IO.Error.mkInterrupted}
+
+{docstring IO.Error.mkInappropriateTypeFile}
+
+# Control Structures
+
+Normally, programs written in {lean}`IO` use {ref "monads-and-do"}[the same control structures as those written in other monads].
+There is one specific {lean}`IO` helper.
+
+{docstring IO.iterate}
+
+{include 0 Manual.IO.Console}
+
+{include 0 Manual.IO.Ref}
+
+{include 0 Manual.IO.Files}
+
+# Environment Variables
+
+{docstring IO.getEnv}
+
+# Timing
+
+{docstring IO.sleep}
+
+{docstring IO.monoNanosNow}
+
+{docstring IO.monoMsNow}
+
+{docstring IO.getNumHeartbeats}
+
+{docstring IO.addHeartbeats}
+
+# Processes
+
+## Current Process
+
+{docstring IO.Process.getCurrentDir}
+
+{docstring IO.Process.setCurrentDir}
+
+{docstring IO.Process.exit}
+
+{docstring IO.Process.getPID}
+
+## Running Processes
+
+There are three primary ways to run other programs from Lean:
+
+ 1. {lean}`IO.Process.run` synchronously executes another program, returning its standard output as a string. It throws an error if the process exits with an error code other than `0`.
+ 2. {lean}`IO.Process.output` synchronously executes another program with an empty standard input, capturing its standard output, standard error, and exit code. No error is thrown if the process terminates unsuccessfully.
+ 3. {lean}`IO.Process.spawn` starts another program asynchronously and returns a data structure that can be used to access the process's standard input, output, and error streams.
+
+{docstring IO.Process.run}
+
+::::example "Running a Program"
+When run, this program concatenates its own source code with itself twice using the Unix tool `cat`.
+
+:::ioExample
+```ioLean
+-- Main.lean begins here
+def main : IO Unit := do
+  let src2 ← IO.Process.run {cmd := "cat", args := #["Main.lean", "Main.lean"]}
+  IO.println src2
+-- Main.lean ends here
+```
+
+Its output is:
+```stdout
+-- Main.lean begins here
+def main : IO Unit := do
+  let src2 ← IO.Process.run {cmd := "cat", args := #["Main.lean", "Main.lean"]}
+  IO.println src2
+-- Main.lean ends here
+-- Main.lean begins here
+def main : IO Unit := do
+  let src2 ← IO.Process.run {cmd := "cat", args := #["Main.lean", "Main.lean"]}
+  IO.println src2
+-- Main.lean ends here
+```
+:::
+::::
+
+::::example "Running a Program on a File"
+
+This program uses the Unix utility `grep` as a filter to find four-digit palindromes.
+It creates a file that contains all numbers from {lean}`0` through {lean}`9999`, and then invokes `grep` on it, reading the result from its standard output.
+
+:::ioExample
+```ioLean
+def main : IO Unit := do
+  -- Feed the input to the subprocess
+  IO.FS.withFile "numbers.txt" .write fun h =>
+    for i in [0:10000] do
+      h.putStrLn (toString i)
+
+  let palindromes ← IO.Process.run {
+    cmd := "grep",
+    args := #[r#"^\([0-9]\)\([0-9]\)\2\1$"#, "numbers.txt"]
+  }
+
+  let count := palindromes.trim.splitOn "\n" |>.length
+
+  IO.println s!"There are {count} four-digit palindromes."
+```
+
+Its output is:
+```stdout
+There are 90 four-digit palindromes.
+```
+:::
+::::
+
+
+{docstring IO.Process.output}
+
+::::example "Checking Exit Codes"
+When run, this program first invokes `cat` on a nonexistent file and displays the resulting error code.
+It then concatenates its own source code with itself twice using the Unix tool `cat`.
+
+:::ioExample
+```ioLean
+-- Main.lean begins here
+def main : IO UInt32 := do
+  let src1 ← IO.Process.output {cmd := "cat", args := #["Nonexistent.lean"]}
+  IO.println s!"Exit code from failed process: {src1.exitCode}"
+
+  let src2 ← IO.Process.output {cmd := "cat", args := #["Main.lean", "Main.lean"]}
+  if src2.exitCode == 0 then
+    IO.println src2.stdout
+  else
+    IO.eprintln "Concatenation failed"
+    return 1
+
+  return 0
+-- Main.lean ends here
+```
+
+Its output is:
+```stdout
+Exit code from failed process: 1
+-- Main.lean begins here
+def main : IO UInt32 := do
+  let src1 ← IO.Process.output {cmd := "cat", args := #["Nonexistent.lean"]}
+  IO.println s!"Exit code from failed process: {src1.exitCode}"
+
+  let src2 ← IO.Process.output {cmd := "cat", args := #["Main.lean", "Main.lean"]}
+  if src2.exitCode == 0 then
+    IO.println src2.stdout
+  else
+    IO.eprintln "Concatenation failed"
+    return 1
+
+  return 0
+-- Main.lean ends here
+-- Main.lean begins here
+def main : IO UInt32 := do
+  let src1 ← IO.Process.output {cmd := "cat", args := #["Nonexistent.lean"]}
+  IO.println s!"Exit code from failed process: {src1.exitCode}"
+
+  let src2 ← IO.Process.output {cmd := "cat", args := #["Main.lean", "Main.lean"]}
+  if src2.exitCode == 0 then
+    IO.println src2.stdout
+  else
+    IO.eprintln "Concatenation failed"
+    return 1
+
+  return 0
+-- Main.lean ends here
+
+```
+:::
+::::
+
+
+{docstring IO.Process.spawn}
+
+::::example "Asynchronous Subprocesses"
+
+This program uses the Unix utility `grep` as a filter to find four-digit palindromes.
+It feeds all numbers from {lean}`0` through {lean}`9999` to the `grep` process and then reads its result.
+This code is only correct when `grep` is sufficiently fast and when the output pipe is large enough to contain all 90 four-digit palindromes.
+
+:::ioExample
+```ioLean
+def main : IO Unit := do
+  let grep ← IO.Process.spawn {
+    cmd := "grep",
+    args := #[r#"^\([0-9]\)\([0-9]\)\2\1$"#],
+    stdin := .piped,
+    stdout := .piped,
+    stderr := .null
+  }
+
+  -- Feed the input to the subprocess
+  for i in [0:10000] do
+    grep.stdin.putStrLn (toString i)
+
+  -- Consume its output, after waiting 100ms for grep to process the data.
+  IO.sleep 100
+  let count := (← grep.stdout.readToEnd).trim.splitOn "\n" |>.length
+
+  IO.println s!"There are {count} four-digit palindromes."
+```
+
+Its output is:
+```stdout
+There are 90 four-digit palindromes.
+```
+:::
+::::
+
+{docstring IO.Process.SpawnArgs}
+
+{docstring IO.Process.StdioConfig}
+
+{docstring IO.Process.Stdio}
+
+{docstring IO.Process.Stdio.toHandleType}
+
+{docstring IO.Process.Child}
+
+{docstring IO.Process.Child.wait}
+
+{docstring IO.Process.Child.tryWait}
+
+{docstring IO.Process.Child.kill}
+
+{docstring IO.Process.Child.takeStdin}
+
+::::example "Closing a Subprocess's Standard Input"
+
+This program uses the Unix utility `grep` as a filter to find four-digit palindromes, ensuring that the subprocess terminates successfully.
+It feeds all numbers from {lean}`0` through {lean}`9999` to the `grep` process, then closes the process's standard input, which causes it to terminate.
+After checking `grep`'s exit code, the program extracts its result.
+
+:::ioExample
+```ioLean
+def main : IO UInt32 := do
+  let grep ← do
+    let (stdin, child) ← (← IO.Process.spawn {
+      cmd := "grep",
+      args := #[r#"^\([0-9]\)\([0-9]\)\2\1$"#],
+      stdin := .piped,
+      stdout := .piped,
+      stderr := .null
+    }).takeStdin
+
+    -- Feed the input to the subprocess
+    for i in [0:10000] do
+      stdin.putStrLn (toString i)
+
+    -- Return the child without its stdin handle.
+    -- This closes the handle, because there are
+    -- no more references to it.
+    pure child
+
+  -- Wait for grep to terminate
+  if (← grep.wait) != 0 then
+    IO.eprintln s!"grep terminated unsuccessfully"
+    return 1
+
+  -- Consume its output
+  let count := (← grep.stdout.readToEnd).trim.splitOn "\n" |>.length
+
+  IO.println s!"There are {count} four-digit palindromes."
+  return 0
+```
+
+Its output is:
+```stdout
+There are 90 four-digit palindromes.
+```
+:::
+::::
+
+{docstring IO.Process.Output}
+
+
+
+# Random Numbers
+
+{docstring IO.setRandSeed}
+
+{docstring IO.rand}
+
+{docstring randBool}
+
+{docstring randNat}
+
+## Random Generators
+
+{docstring RandomGen}
+
+{docstring StdGen}
+
+{docstring stdRange}
+
+{docstring stdNext}
+
+{docstring stdSplit}
+
+{docstring mkStdGen}
+
+## System Randomness
+
+{docstring IO.getRandomBytes}
+
+{include 0 Manual.IO.Threads}
