Manual/IO/Console.lean
@@ -1,0 +1,64 @@
+/-
+Copyright (c) 2024 Lean FRO LLC. All rights reserved.
+Released under Apache 2.0 license as described in the file LICENSE.
+Author: David Thrane Christiansen
+-/
+
+import VersoManual
+
+import Manual.Meta
+
+import Lean.Parser.Command
+
+open Manual
+open Verso.Genre
+open Verso.Genre.Manual
+
+set_option pp.rawOnError true
+
+set_option linter.unusedVariables false
+
+#doc (Manual) "Console Output" =>
+
+Lean includes convenience functions for writing to {tech}[standard output] and {tech}[standard error].
+All make use of {lean}`ToString` instances, and the varieties whose names end in `-ln` add a newline after the output.
+These convenience functions only expose a part of the functionality available {ref "stdio"}[using the standard I/O streams].
+In particular, to read a line from standard input, use a combination of {lean}`IO.getStdin` and {lean}`IO.FS.Stream.getLine`.
+
+{docstring IO.print}
+
+{docstring IO.println}
+
+{docstring IO.eprint}
+
+{docstring IO.eprintln}
+
+::::example "Printing"
+This program demonstrates all four convenience functions for console I/O.
+
+:::ioExample
+```ioLean
+def main : IO Unit := do
+  IO.print "This is the "
+  IO.print "Lean"
+  IO.println " language reference."
+  IO.println "Thank you for reading it!"
+  IO.eprint "Please report any "
+  IO.eprint "errors"
+  IO.eprintln " so they can be corrected."
+```
+
+It outputs the following to the standard output:
+
+```stdout
+This is the Lean language reference.
+Thank you for reading it!
+```
+
+and the following to the standard error:
+
+```stderr
+Please report any errors so they can be corrected.
+```
+:::
+::::
