Manual/IO/Ref.lean
@@ -1,0 +1,223 @@
+/-
+Copyright (c) 2024 Lean FRO LLC. All rights reserved.
+Released under Apache 2.0 license as described in the file LICENSE.
+Author: David Thrane Christiansen
+-/
+
+import VersoManual
+
+import Manual.Meta
+import Manual.Papers
+
+import Lean.Parser.Command
+
+open Manual
+open Verso.Genre
+open Verso.Genre.Manual
+
+set_option pp.rawOnError true
+
+set_option linter.unusedVariables false
+
+#doc (Manual) "Mutable References" =>
+
+
+While ordinary {tech}[state monads] encode stateful computations with tuples that track the contents of the state along with the computation's value, Lean's runtime system also provides mutable references that are always backed by mutable memory cells.
+Mutable references have a type {lean}`IO.Ref` that indicates that a cell is mutable, and reads and writes must be explicit.
+{lean}`IO.Ref` is implemented using {lean}`ST.Ref`, so the entire {ref "mutable-st-references"}[{lean}`ST.Ref` API] may also be used with {lean}`IO.Ref`.
+
+{docstring IO.Ref}
+
+{docstring IO.mkRef}
+
+
+
+# State Transformers
+%%%
+tag := "mutable-st-references"
+%%%
+
+
+Mutable references are often useful in contexts where arbitrary side effects are undesired.
+They can give a significant speedup when Lean is unable to optimize pure operations into mutation, and some algorithms are more easily expressed using mutable references than with state monads.
+Additionally, it has a property that other side effects do not have: if all of the mutable references used by a piece of code are created during its execution, and no mutable references from the code escape to other code, then the result of evaluation is deterministic.
+
+The {lean}`ST` monad is a restricted version of {lean}`IO` in which mutable state is the only side effect, and mutable references cannot escape.{margin}[{lean}`ST` was first described by {citehere launchbury94}[].]
+{lean}`ST` takes a type parameter that is never used to classify any terms.
+The {lean}`runST` function, which allow escape from {lean}`ST`, requires that the {lean}`ST` action that is passed to it can instantiate this type parameter with _any_ type.
+This unknown type does not exist except as a parameter to a function, which means that values whose types are “marked” by it cannot escape its scope.
+
+{docstring ST}
+
+{docstring runST}
+
+As with {lean}`IO` and {lean}`EIO`, there is also a variation of {lean}`ST` that takes a custom error type as a parameter.
+Here, {lean}`ST` is analogous to {lean}`BaseIO` rather than {lean}`IO`, because {lean}`ST` cannot result in errors being thrown.
+
+{docstring EST}
+
+{docstring runEST}
+
+{docstring ST.Ref}
+
+{docstring ST.mkRef}
+
+## Reading and Writing
+
+{docstring ST.Ref.get}
+
+{docstring ST.Ref.set}
+
+::::example "Data races with {name ST.Ref.get}`get` and {name ST.Ref.set}`set`"
+:::ioExample
+```ioLean
+def main : IO Unit := do
+  let balance ← IO.mkRef (100 : Int)
+
+  let mut orders := #[]
+  IO.println "Sending out orders..."
+  for _ in [0:100] do
+    let o ← IO.asTask (prio := .dedicated) do
+      let cost ← IO.rand 1 100
+      IO.sleep (← IO.rand 10 100).toUInt32
+      if cost < (← balance.get) then
+        IO.sleep (← IO.rand 10 100).toUInt32
+        balance.set ((← balance.get) - cost)
+    orders := orders.push o
+
+  -- Wait until all orders are completed
+  for o in orders do
+    match o.get with
+    | .ok () => pure ()
+    | .error e => throw e
+
+  if (← balance.get) < 0 then
+    IO.eprintln "Final balance is negative!"
+  else
+    IO.println "Final balance is zero or positive."
+```
+```stdout
+Sending out orders...
+```
+```stderr
+Final balance is negative!
+```
+:::
+::::
+
+{docstring ST.Ref.modify}
+
+::::example "Avoiding data races with {name ST.Ref.modify}`modify`"
+
+This program launches 100 threads.
+Each thread simulates a purchase attempt: it generates a random price, and if the account balance is sufficient, it decrements it by the price.
+The balance check and the computation of the new value occur in an atomic call to {name}`ST.Ref.modify`.
+
+:::ioExample
+```ioLean
+def main : IO Unit := do
+  let balance ← IO.mkRef (100 : Int)
+
+  let mut orders := #[]
+  IO.println "Sending out orders..."
+  for _ in [0:100] do
+    let o ← IO.asTask (prio := .dedicated) do
+      let cost ← IO.rand 1 100
+      IO.sleep (← IO.rand 10 100).toUInt32
+      balance.modify fun b =>
+        if cost < b then
+          b - cost
+        else b
+    orders := orders.push o
+
+  -- Wait until all orders are completed
+  for o in orders do
+    match o.get with
+    | .ok () => pure ()
+    | .error e => throw e
+
+  if (← balance.get) < 0 then
+    IO.eprintln "Final balance negative!"
+  else
+    IO.println "Final balance is zero or positive."
+```
+```stdout
+Sending out orders...
+Final balance is zero or positive.
+```
+```stderr
+```
+:::
+::::
+
+{docstring ST.Ref.modifyGet}
+
+## Comparisons
+
+{docstring ST.Ref.ptrEq}
+
+## Concurrency
+
+Mutable references can be used as a locking mechanism.
+_Taking_ the contents of the reference causes attempts to take it or to read from it to block until it is {name ST.Ref.set}`set` again.
+This is a low-level feature that can be used to implement other synchronization mechanisms; it's usually better to rely on higher-level abstractions when possible.
+
+{docstring ST.Ref.take}
+
+{docstring ST.Ref.swap}
+
+{docstring ST.Ref.toMonadStateOf}
+
+
+::::example "Reference Cells as Locks"
+This program launches 100 threads.
+Each thread simulates a purchase attempt: it generates a random price, and if the account balance is sufficient, it decrements it by the price.
+If the balance is not sufficient, then it is not decremented.
+Because each thread {name ST.Ref.take}`take`s the balance cell prior to checking it and only returns it when it is finished, the cell acts as a lock.
+Unlike using {name}`ST.Ref.modify`, which atomically modifies the contents of the cell using a pure function, other {name}`IO` actions may occur in the critical section
+This program's `main` function is marked {keywordOf Lean.Parser.Command.declaration}`unsafe` because {name ST.Ref.take}`take` itself is unsafe.
+
+:::ioExample
+```ioLean
+unsafe def main : IO Unit := do
+  let balance ← IO.mkRef (100 : Int)
+  let validationUsed ← IO.mkRef false
+
+  let mut orders := #[]
+
+  IO.println "Sending out orders..."
+  for _ in [0:100] do
+    let o ← IO.asTask (prio := .dedicated) do
+      let cost ← IO.rand 1 100
+      IO.sleep (← IO.rand 10 100).toUInt32
+      let b ← balance.take
+      if cost ≤ b then
+        balance.set (b - cost)
+      else
+        balance.set b
+        validationUsed.set true
+    orders := orders.push o
+
+  -- Wait until all orders are completed
+  for o in orders do
+    match o.get with
+    | .ok () => pure ()
+    | .error e => throw e
+
+  if (← validationUsed.get) then
+    IO.println "Validation prevented a negative balance."
+
+  if (← balance.get) < 0 then
+    IO.eprintln "Final balance negative!"
+  else
+    IO.println "Final balance is zero or positive."
+```
+
+The program's output is:
+```stdout
+Sending out orders...
+Validation prevented a negative balance.
+Final balance is zero or positive.
+```
+:::
+::::
