Manual/IO/Threads.lean
@@ -1,0 +1,84 @@
+/-
+Copyright (c) 2024 Lean FRO LLC. All rights reserved.
+Released under Apache 2.0 license as described in the file LICENSE.
+Author: David Thrane Christiansen
+-/
+
+import VersoManual
+
+import Manual.Meta
+
+import Lean.Parser.Command
+
+open Manual
+open Verso.Genre
+open Verso.Genre.Manual
+
+set_option pp.rawOnError true
+
+set_option linter.unusedVariables false
+
+#doc (Manual) "Tasks and Threads" =>
+
+::: planned 90
+A detailed description of the Lean multi-threading model, including:
+
+ * {lean}`Task`s, priorities, and threads
+ * Synchronization and communication primitives
+    * {lean}`IO.Ref` as a lock
+    * {lean}`IO.Mutex`
+    * {lean}`IO.Channel`
+    * {lean}`IO.Condvar`
+    * {lean}`IO.Promise`
+:::
+
+
+{docstring Task}
+
+{docstring Task.spawn}
+
+{docstring Task.Priority}
+
+{docstring Task.Priority.default}
+
+{docstring Task.Priority.max}
+
+{docstring Task.Priority.dedicated}
+
+{docstring Task.get}
+
+{docstring IO.wait}
+
+{docstring IO.waitAny}
+
+{docstring BaseIO.mapTask}
+
+{docstring EIO.mapTask}
+
+{docstring IO.mapTask}
+
+{docstring BaseIO.mapTasks}
+
+{docstring EIO.mapTasks}
+
+{docstring IO.mapTasks}
+
+{docstring BaseIO.bindTask}
+
+{docstring EIO.bindTask}
+
+{docstring IO.bindTask}
+
+{docstring BaseIO.asTask}
+
+{docstring EIO.asTask}
+
+{docstring IO.asTask}
+
+{docstring IO.cancel}
+
+{docstring IO.getTaskState}
+
+{docstring IO.checkCanceled}
+
+{docstring IO.hasFinished}
