Manual/Meta.lean
@@ -23,6 +23,7 @@ import Manual.Meta.CustomStyle
 import Manual.Meta.Example
 import Manual.Meta.Figure
 import Manual.Meta.Lean
+import Manual.Meta.Lean.IO
 import Manual.Meta.Marginalia
 import Manual.Meta.ParserAlias
 import Manual.Meta.Syntax
